kjrgnekrjf

LeanGrow/Src/Utils/Lean/Proofs/Subterms.lean
@@ -5,10 +5,8 @@ Released under Apache 2.0 license as described in the file LICENSE.
 Author: Yves Jäckle.
 -/
 
-import LeanGrow.Src.Utils.Tracing
-import LeanGrow.Src.Utils.Lean.LocalContext
-import LeanGrow.Src.Utils.Lean.Expr.Fail
-import LeanGrow.Src.Utils.LeanGrow.Nodes
+import LeanGrow.Src.Utils.Lean.Expr.Basic
+import Lean
 
 open Lean Meta
 
@@ -29,9 +27,9 @@ def mkValLikeCore (n : Name) : MetaM Unit := do
   }
   addDecl dec
 
-elab "add_valLike" n:ident : command => do
-  let N := n.getId
-  Elab.Command.liftTermElabM (mkValLikeCore N)
+-- elab "add_valLike" n:ident : command => do
+--   let N := n.getId
+--   Elab.Command.liftTermElabM (mkValLikeCore N)
 
 elab "ppElabOf" t:term : term => do
   let t ← Elab.Term.elabTermAndSynthesize t .none
@@ -39,39 +37,6 @@ elab "ppElabOf" t:term : term => do
   return t
 
 #check 1
-
-
-@[specialize f, inline]
-partial def Lean.Expr.onAllSubtermsWiDepth (e : Expr) (f : Expr → Nat → Expr) : Expr :=
-  -- caching here is bad idea because cached term can appear in different depths,
-  -- and bvar indices will be wrong there. This happend.
-  let rec @[specialize f] go (e : Expr) (d : Nat) : Expr :=
-    match f e d with
-    | .app l r =>
-      let l := go l d
-      let r := go r d
-      .app l r
-    | .lam n l r bi =>
-      let l := go l d
-      let r := go r (d+1)
-      .lam n l r bi
-    | .forallE n l r bi =>
-      let l := go l d
-      let r := go r (d+1)
-      .forallE n l r bi
-    | .letE n l r z bi =>
-      let l := go l d
-      let r := go r d
-      let z := go z (d+1)
-      .letE n l r z bi
-    | .proj n i l =>
-      let l := go l d
-      .proj n i l
-    | .mdata da l =>
-      let l := go l d
-      .mdata da l
-    | t => t
-  go e 0
 
 open Elab Term
 
@@ -81,69 +46,305 @@ def help : Expr → TermElabM FVarId
   | .fvar i => return i
   | _ => throwError "bad format"
 
-@[specialize f,inline]
-partial def Lean.Level.onAllSubtermsFold (e : Level)
-  {α : Sort _} (init : α) (f : Level → α → α) : α :=
-  let rec @[specialize f] go (col : α) : Level → α
-    | e  =>
-      let here := f e col
-      match e with
-      | .max l r | .imax l r => let nx := go here l ; go nx r
-      | .succ e => go (here) e
-      | _ => here
-  go init e
 
-def mkValLikeCore' (fu body : Expr) : TermElabM Unit := do
+@[inline]
+partial def Lean.Expr.abstractLetFvarLam'
+  (initD : LocalContext) (initI : LocalInstances)
+  (fvs : Array FVarId) (e : Expr)
+  : MetaM (Prod3 Expr LocalContext LocalInstances) :=
+    let rec bind (term : Expr) (i : Nat) (initD : LocalContext) (initI : LocalInstances) : MetaM (Prod3 Expr LocalContext LocalInstances) := do
+     dbg_trace s!"bind {repr (fvs[i]!)}"
+      match ← (fvs[i]!).GetDecl initD initI with
+      | .cdecl _ _ _ T .. =>
+          let ⟨T,initD,initI⟩ ← T.onAllSubtermsM initD initI (fun x d initD initI =>
+            match x with
+            | .fvar id =>
+              match fvs.findIdx? (fun y => y == id) with
+              | .none => return ⟨x,initD,initI⟩
+              | .some j => return ⟨(.bvar (d + i - 1 - j)),initD,initI⟩
+            | _ => return ⟨x,initD,initI⟩ )
+          if i == 0
+          then
+            match ← IsClass? T initD initI with
+            | .none => return ⟨.lam `abstractFvarWrt T term .default,initD,initI⟩
+            | _ => return ⟨.lam `abstractFvarWrt T term .instImplicit,initD,initI⟩
+          else
+            match ← IsClass? T initD initI with
+            | .none => bind (.lam `abstractFvarWrt T term .default) (i-1) initD initI
+            | _ => bind (.lam `abstractFvarWrt T term .instImplicit) (i-1) initD initI
+      | .ldecl _ _ _ T V nonDep .. =>
+          let ⟨T,initD,initI⟩ ← T.onAllSubtermsM initD initI (fun x d initD initI =>
+            match x with
+            | .fvar id =>
+              match fvs.findIdx? (fun y => y == id) with
+              | .none => return ⟨x,initD,initI⟩
+              | .some j => return ⟨(.bvar (d + i - 1 - j)),initD,initI⟩
+            | _ => return ⟨x,initD,initI⟩ )
+          if i == 0
+          then
+            return ⟨.letE `abstractFvarWrt T V term nonDep,initD,initI⟩
+          else
+            bind (.letE `abstractFvarWrt T V term nonDep) (i-1) initD initI
+    do
+    let fvS := fvs.size
+    if fvS == 0
+    then return ⟨e,initD,initI⟩
+    else
+      let ⟨absd,initD,initI⟩ ← e.onAllSubtermsM initD initI (fun x d initD initI =>
+        match x with
+        | .fvar id =>
+          match fvs.findIdx? (fun y => y == id) with
+          | .none => return ⟨x,initD,initI⟩
+          | .some i => return ⟨(.bvar (d + fvS - 1 - i)),initD,initI⟩
+        | _ => return ⟨x,initD,initI⟩ )
+      dbg_trace "passed abs"
+      bind absd (fvs.size - 1) initD initI
+
+
+-- #exit
+
+def mkValLikeCore' (fu body : Expr) (args : Array Expr) : TermElabM Unit := do
   let fv ← help fu
+  logInfoAt (← getRef) s!"fu : {← ppExpr fu}\n{fu}"
+  logInfoAt (← getRef) s!"args : {repr args}"
   let N ← fv.getUserName
   let N := Name.str N "like"
-  let (_,allFv) ←  body.collectFVars.run {}
-  let absed := body.abstract (allFv.fvarIds.map Expr.fvar) -- ignores dependencies
-  -- bindddmfnrjngqöejn
+  let args := args.map Expr.fvarId!
+  logInfoAt (← getRef) s!"sanity 1 : {repr <| body.getFVarIds}"
+  logInfoAt (← getRef) s!"sanity 2 : {repr <| (← getLCtx).decls.toArray.map (fun x => x.map (fun y => (y.fvarId, y.userName)))}"
+  let .mk absed _ _ ← Lean.Expr.abstractLetFvarLam' (← getLCtx) (← getLocalInstances) args body -- ignores dependencies
+  logInfoAt (← getRef) s!"absed : {← ppExpr absed}\n{absed}"
   let T ← inferType fu
+  logInfoAt (← getRef) s!"T : {← ppExpr T}\n{T}"
   let lv ← getLevel T
-  let eq := mkAppN (.const ``Eq [lv]) #[T,(.bvar 0), absed]
-  let lvl := lv.onAllSubtermsFold [] (fun | .param n, s => s.insert n | _,s => s) -- not in right order ...
-  let eq := Expr.lam `f T eq .default
+  logInfoAt (← getRef) s!"Lv : {lv}"
+  let eq := mkAppN (.const ``Eq [lv]) #[T, Expr.fvar fv, absed]
+  let lvl := lv.onAllSubtermsFold [] (fun | .param n, s => s.insert n | _,s => s)
+  let .mk eq _ _ ← Lean.Expr.abstractLetFvarLam (← getLCtx) (← getLocalInstances) #[fv] eq
+  logInfoAt (← getRef) s!"eq : {← ppExpr eq}\n{eq}"
   let dec : Declaration := .defnDecl <| {
     name := N
     levelParams := lvl
-    type := .sort 0
+    type := Expr.forallE N T (.sort 0) .default
     value := eq
     hints := .regular 0
     safety := .safe
   }
   addDecl dec
 
+#check mkLambdaFVars
+#check Expr.cleanupAnnotations
 
-elab "add_valLike_of" fu:term "in" body:term : term => do
+def Lean.Expr.cleanupAnnotations! (e : Expr) :=
+  Lean.Expr.onAllSubtermsWiDepth e (fun x _ => x.cleanupAnnotations)
+
+
+-- #exit
+
+elab "add_valLike" fu:term "args" as:term,* "in" body:term : term => do
   let fu ← Elab.Term.elabTermAndSynthesize fu .none
+  let fu := fu.cleanupAnnotations!
+  let as := as.getElems
+  let args ← as.mapM (Elab.Term.elabTermAndSynthesize · .none)
+  let args := args.map .cleanupAnnotations!
   let body ← Elab.Term.elabTermAndSynthesize body .none
-  mkValLikeCore' fu body
+  let body' := body.cleanupAnnotations!
+  mkValLikeCore' fu body' args
+  logInfoAt (← getRef) s!"{← getDeclName?}"
   return body
 
 
 #check Meta.getLevel
+#check mkLambdaFVars
 
-#exit
+
+-- #exit
 
 @[specialize f]
-partial def Lean.Expr.onAllSubterms (e : Expr) (f : Expr → Expr) : Expr :=
-  let rec @[specialize f] go (e : Expr) : Expr :=
+partial def Lean.Expr.onAllSubterms' (e : Expr) (f : Expr → Expr) : Expr :=
+  let rec @[specialize f] go (f : Expr → Expr)  (e : Expr) : Expr :=
     -- ppElabOf
-    add_valLike_of go in
-    let here := f e
-    match here with
-    | .app l r => Expr.app (go l) (go r)
-    | .lam n l r i => .lam n (go l) (go r)  i
-    | .forallE n l r i => .forallE n (go l) (go r)  i
-    | .letE n l r z i => .letE n (go l) (go r) (go z)  i
-    | .proj n i e => .proj n i (go e)
-    | .mdata d e => .mdata d (go e)
-    | _ => here
-  go e
+    add_valLike go args f, e in
+    match f e with
+    | .app l r => Expr.app (go f l) (go f r)
+    | .lam n l r i => .lam n (go f l) (go f r)  i
+    | .forallE n l r i => .forallE n (go f l) (go f r)  i
+    | .letE n l r z i => .letE n (go f l) (go f r) (go f z)  i
+    | .proj n i e => .proj n i (go f e)
+    | .mdata d e => .mdata d (go f e)
+    | here => here
+  go f e
 
 -- add_valLike Lean.Expr.onAllSubterms.go
 -- has no val you dummy
 
 #check 1
+#print go.like
+
+
+#print DefinitionSafety
+
+#check Environment.isSafeDefinition
+#print DefinitionVal
+
+
+#check Elab.Term.getDeclName?
+
+#check mkInductiveDeclEs
+#print InductiveType
+#print Constructor
+
+/- todo:
+- use elab decl name instead of fvar name
+- look for patial consts in body and check if env have like-principles
+  for them, and add them as fields to the structure that is the cuurently
+  built like-principle
+
+-/
+
+#check Expr.rec
+
+
+-- def OnAllSub (P : Expr → Prop) (e : Expr) :=
+--   P e ∧
+--     match e with
+--     | .app l r => P l ∧ P r
+--     | .lam _ l r _ => P l ∧ P r
+--     | .forallE _ l r _ => P l ∧ P r
+--     | .letE _ l r z _ => P l ∧ P r ∧ P z
+--     | .proj _ _ e => P e
+--     | .mdata _ e => P e
+--     | _ => True
+
+
+-- example (f : Expr → Expr) (g : (Expr → Expr) → Expr → Expr)
+--   (h_g : go.like g)
+--   {P : Expr → Prop}
+--   (h_f :∀ e, P (f e))
+--   (app : (fn arg : Expr) → P fn → P arg → P (fn.app arg))
+--   (lam :
+--     (binderName : Name) →
+--       (binderType body : Expr) →
+--         (binderInfo : BinderInfo) →
+--           P binderType → P body → P (Expr.lam binderName binderType body binderInfo))
+--   (forallE :
+--     (binderName : Name) →
+--       (binderType body : Expr) →
+--         (binderInfo : BinderInfo) →
+--           P binderType → P body → P (Expr.forallE binderName binderType body binderInfo))
+--   (letE :
+--     (declName : Name) →
+--       (type value body : Expr) →
+--         (nondep : Bool) → P type → P value → P body → P (Expr.letE declName type value body nondep))
+--   (mdata : (data : MData) → (expr : Expr) → P expr → P (Expr.mdata data expr))
+--   (proj : (typeName : Name) → (idx : Nat) → (struct : Expr) → P struct → P (Expr.proj typeName idx struct))
+--   : ∀ e, P (g f e) := by
+--       intro e
+--       rw [h_g]
+--       let fe := f e
+--       have fed : fe = f e := rfl
+--       dsimp
+--       rw [← fed]
+--       revert fed
+--       induction fe with
+--       | bvar => dsimp ; intro fed ; rw [fed] ; apply h_f
+--       | fvar => dsimp ; intro fed ; rw [fed] ; apply h_f
+--       | mvar => dsimp ; intro fed ; rw [fed] ; apply h_f
+--       | const => dsimp ; intro fed ; rw [fed] ; apply h_f
+--       | lit => dsimp ; intro fed ; rw [fed] ; apply h_f
+--       | app l r il ir =>
+
+      -- have :=
+      --   @Expr.rec
+      --     (fun x =>
+      --       match x with
+      --       | .bvar .. | .fvar .. | .mvar .. | .sort .. | .const .. | .lit .. =>
+      --         x = f e →
+      --           P (match x with
+      --               | .app l r => (g f l).app (g f r)
+      --               | Expr.lam n l r i => Expr.lam n (g f l) (g f r) i
+      --               | Expr.forallE n l r i => Expr.forallE n (g f l) (g f r) i
+      --               | Expr.letE n l r z i => Expr.letE n (g f l) (g f r) (g f z) i
+      --               | Expr.proj n i e => Expr.proj n i (g f e)
+      --               | Expr.mdata d e => Expr.mdata d (g f e)
+      --               | here => here)
+      --       | _ =>
+      --         P (match x with
+      --             | .app l r => (g f l).app (g f r)
+      --             | Expr.lam n l r i => Expr.lam n (g f l) (g f r) i
+      --             | Expr.forallE n l r i => Expr.forallE n (g f l) (g f r) i
+      --             | Expr.letE n l r z i => Expr.letE n (g f l) (g f r) (g f z) i
+      --             | Expr.proj n i e => Expr.proj n i (g f e)
+      --             | Expr.mdata d e => Expr.mdata d (g f e)
+      --             | here => here)
+      --       )
+      --     (fun _ => by dsimp ; intro fed ; rw [fed] ; apply h_f)
+      --     (fun _ => by dsimp ; intro fed ; rw [fed] ; apply h_f)
+      --     (fun _ => by dsimp ; intro fed ; rw [fed] ; apply h_f)
+      --     (fun _ => by dsimp ; intro fed ; rw [fed] ; apply h_f)
+      --     (fun _ _ => by dsimp ; intro fed ; rw [fed] ; apply h_f)
+      --     (fun l r il ir => by
+      --       dsimp at ⊢ il ir
+      --       )
+
+
+      -- suffices H : OnAllSub P (g f e) from H.1
+      -- rw [h_g]
+      -- let fe := f e
+      -- have fed : fe = f e := rfl
+      -- dsimp
+      -- rw [← fed]
+      -- revert fed
+      -- induction fe with
+      -- | bvar =>
+      --   dsimp ; intro fed ; unfold OnAllSub
+      --   constructor
+      --   · rw [fed] ; apply h_f
+      --   · dsimp
+      -- | fvar =>
+      --   dsimp ; intro fed ; unfold OnAllSub
+      --   constructor
+      --   · rw [fed] ; apply h_f
+      --   · dsimp
+      -- | mvar =>
+      --   dsimp ; intro fed ; unfold OnAllSub
+      --   constructor
+      --   · rw [fed] ; apply h_f
+      --   · dsimp
+      -- | sort =>
+      --   dsimp ; intro fed ; unfold OnAllSub
+      --   constructor
+      --   · rw [fed] ; apply h_f
+      --   · dsimp
+      -- | const =>
+      --   dsimp ; intro fed ; unfold OnAllSub
+      --   constructor
+      --   · rw [fed] ; apply h_f
+      --   · dsimp
+      -- | app l r il ir =>
+      --   intro q
+      --   dsimp
+      --   unfold OnAllSub at *
+
+
+--add_valLike go args f, e in
+
+partial def test1 (n : Nat) : Nat :=
+  add_valLike test1 args n in
+  test1 (n+1)
+
+
+#print test1.like
+
+
+example (f : Nat → Nat) (h : test1.like f)
+  : ∃ c, f = (fun _ => c) := by
+    let x := f 0
+    refine ⟨x, ?_⟩
+    funext n
+    induction n with
+    | zero => rfl
+    | succ n ih =>
+      rw [h] at ih
+      dsimp at ih
+      exact ih
